theories/std/assume.v
@@ -1,0 +1,36 @@
+From ml Require Import
+  prelude.
+From ml.language Require Import
+  notations
+  proofmode.
+From ml.std Require Export
+  base.
+From ml.std Require Import
+  diverge.
+
+Definition assume : val :=
+  λ: "b",
+    if: "b" then #() else diverge #().
+
+Section heapGS.
+  Context `{!heapGS Σ}.
+
+  Lemma assume_spec (b : bool) Φ :
+    ▷ (⌜b = true⌝ → Φ #()) -∗
+    WP assume #b {{ Φ }}.
+  Proof.
+    iIntros "HΦ".
+    wp_rec. destruct b; first iSmash.
+    wp_smart_apply wp_diverge.
+  Qed.
+  Lemma assume_spec' ϕ `{!Decision ϕ} Φ :
+    ▷ (⌜ϕ⌝ → Φ #()) -∗
+    WP assume #(bool_decide ϕ) {{ Φ }}.
+  Proof.
+    iIntros "HΦ".
+    wp_apply assume_spec. iIntros (Hϕ%bool_decide_eq_true_1).
+    iSmash.
+  Qed.
+End heapGS.
+
+#[global] Opaque assume.
